documentation for CSR_float

experiments/CSR_float.v
@@ -42,6 +42,7 @@ Tactic Notation "seclocal_solver" :=
 
 Definition indexf := index_bounded.func.
 
+(* Float version of `sv.get` *)
 Definition get := 
   <{
   fun i xind xval xlb xrb =>
@@ -56,11 +57,11 @@ Lemma get_spec_in {D : Type} `{Inhab D} (x_ind x_val : loc) i d :
   @htriple D (single d tt) 
     (fun=> get (List.nth (abs i) (xind [[ lb -- rb ]]) 0) x_ind x_val lb rb)
     (\[0 <= i < N] \*
-      harray_int xind x_ind d \* 
+      arr(x_ind, xind)⟨`d⟩ \* 
       harray_float xval x_val d)
     (fun hr => 
      \[hr = fun=> List.nth (abs i) (xval [[ lb -- rb ]]) float_unit] \* 
-      harray_int xind x_ind d \* 
+      arr(x_ind, xind)⟨`d⟩ \* 
       harray_float xval x_val d).
 Proof with seclocal_solver.
   xwp; xsimpl=> ?; xapp (@index_bounded.spec _ H)=> //.
@@ -69,15 +70,15 @@ Proof with seclocal_solver.
   xapp; xsimpl*...
 Qed.
 
-Lemma get_spec_out_unary {D : Type} `{Inhab D} (x_ind x_val : loc) (i : int) d : 
-  @htriple D (single d tt) 
+Lemma get_spec_out_unary {D : Type} `{Inhab D} (x_ind x_val : loc) (i : int) (d : D) : 
+  htriple (`{d}) 
     (fun=> get i x_ind x_val lb rb)
     (\[~ In i (xind [[ lb -- rb ]])] \*
-      harray_int xind x_ind d \* 
+      arr(x_ind, xind)⟨`d⟩ \* 
       harray_float xval x_val d)
     (fun hr => 
      \[hr = fun=> float_unit] \* 
-      harray_int xind x_ind d \* 
+      arr(x_ind, xind)⟨`d⟩ \* 
       harray_float xval x_val d).
 Proof.
   xwp; xsimpl=> ?; xapp (@index_bounded.spec _ H)=> //...
@@ -87,15 +88,15 @@ Qed.
 
 Local Notation D := (labeled int).
 
-Lemma get_spec_out `{Inhab D} fs (x_ind x_val : loc) : 
-  @htriple D fs
+Lemma get_spec_out `{Inhab D} (fs : fset D) (x_ind x_val : loc) : 
+  htriple fs
     (fun i => get (eld i) x_ind x_val lb rb)
     (\[forall d, indom fs d -> ~ In (eld d) (xind [[ lb -- rb ]])] \*
-      (\*_(d <- fs) harray_int xind x_ind d) \* 
+      (\*_(d <- fs) arr(x_ind, xind)⟨`d⟩) \* 
        \*_(d <- fs) harray_float xval x_val d)
     (fun hr => 
      \[hr = fun=> float_unit] \* 
-      ((\*_(d <- fs) harray_int xind x_ind d) \* 
+      ((\*_(d <- fs) arr(x_ind, xind)⟨`d⟩) \* 
        \*_(d <- fs) harray_float xval x_val d)).
 Proof. by xpointwise_build (@get_spec_out_unary). Qed.
 
@@ -108,8 +109,8 @@ Module csr_float.
 Section csr.
 
 Notation "'mval'" := ("m_val":var) (in custom trm at level 0) : trm_scope.
-Notation "'colind'" := ("col_ind":var) (in custom trm at level 0) : trm_scope.
-Notation "'rowptr'" := ("row_ptr":var) (in custom trm at level 0) : trm_scope.
+Notation "'mind'" := ("m_ind":var) (in custom trm at level 0) : trm_scope.
+Notation "'mcrd'" := ("m_crd":var) (in custom trm at level 0) : trm_scope.
 Notation "'dvec'" := ("d_vec":var) (in custom trm at level 0) : trm_scope.
 Notation "'lb'" := ("l_b":var) (in custom trm at level 0) : trm_scope.
 Notation "'rb'" := ("r_b":var) (in custom trm at level 0) : trm_scope.
@@ -118,49 +119,49 @@ Notation "'i''" := ("i_'":var) (in custom trm at level 0) : trm_scope.
 Import List Vars list_interval_notation.
 
 Context (mval : list binary64).
-Context (colind rowptr : list int).
+Context (mind mcrd : list int).
 Context (N Nrow Ncol : int).
 Hypothesis Nrow_nonneg : 0 <= Nrow.
 Hypothesis len_mval : length mval = N :> int.
-Hypothesis len_colind : length colind = N :> int.
-Hypothesis len_rowptr : length rowptr = Nrow + 1 :> int.
-Hypothesis colind_leq : forall x, In x colind -> 0 <= x < Ncol.
-Hypothesis rowptr_first : List.nth (abs 0) rowptr 0 = 0.
-Hypothesis rowptr_last : List.nth (abs Nrow) rowptr 0 = N.
-Hypothesis rowptr_weakly_sorted : forall (i j : int), 
+Hypothesis len_mind : length mind = N :> int.
+Hypothesis len_mcrd : length mcrd = Nrow + 1 :> int.
+Hypothesis mind_leq : forall x, In x mind -> 0 <= x < Ncol.
+Hypothesis mcrd_first : List.nth (abs 0) mcrd 0 = 0.
+Hypothesis mcrd_last : List.nth (abs Nrow) mcrd 0 = N.
+Hypothesis mcrd_weakly_sorted : forall (i j : int), 
   (0 <= i <= Nrow) -> 
   (0 <= j <= Nrow) -> 
   (i <= j) -> 
-  (rowptr[i] <= rowptr[j]).
+  (mcrd[i] <= mcrd[j]).
 Hypothesis mval_finite : forall x, In x mval -> @finite Tdouble x.
 
-Definition colind_seg (row : int) := colind [[ (rowptr[row]) -- (rowptr[row + 1]) ]].
+Definition mind_seg (row : int) := mind [[ (mcrd[row]) -- (mcrd[row + 1]) ]].
 
-Hypothesis nodup_eachcol : forall x : int, 0 <= x < Nrow -> NoDup (colind_seg x).
-Hypothesis sorted_eachcol : forall x : int, 0 <= x < Nrow -> sorted (colind_seg x). 
+Hypothesis nodup_eachcol : forall x : int, 0 <= x < Nrow -> NoDup (mind_seg x).
+Hypothesis sorted_eachcol : forall x : int, 0 <= x < Nrow -> sorted (mind_seg x). 
 
 Local Tactic Notation "seclocal_solver" :=
   first [ assumption 
-    | rewrite -/(colind_seg _); now apply nodup_eachcol
-    | (* for rowptr[?] <= N *)
-      try rewrite -> len_colind; try rewrite -> len_mval; 
-      try rewrite <- rowptr_last; apply rowptr_weakly_sorted; math
-    | (* for 0 <= rowptr[?] *)
-      rewrite <- rowptr_first at 1; apply rowptr_weakly_sorted; math
-    | (* for 0 <= rowptr[i] <= rowptr[i + 1] *)
-      split; [ rewrite <- rowptr_first at 1 | ]; apply rowptr_weakly_sorted; math
+    | rewrite -/(mind_seg _); now apply nodup_eachcol
+    | (* for mcrd[?] <= N *)
+      try rewrite -> len_mind; try rewrite -> len_mval; 
+      try rewrite <- mcrd_last; apply mcrd_weakly_sorted; math
+    | (* for 0 <= mcrd[?] *)
+      rewrite <- mcrd_first at 1; apply mcrd_weakly_sorted; math
+    | (* for 0 <= mcrd[i] <= mcrd[i + 1] *)
+      split; [ rewrite <- mcrd_first at 1 | ]; apply mcrd_weakly_sorted; math
       (* TODO this could be better? *)
-    | intros; eapply colind_leq, in_interval_list; now eauto
+    | intros; eapply mind_leq, in_interval_list; now eauto
     | intros; eapply mval_finite, in_interval_list; now eauto
     | idtac ]; auto.
 
 Definition get := 
 <{
-  fun mval colind rowptr i j =>
-    let lb = read_array rowptr i in
+  fun mval mind mcrd i j =>
+    let lb = read_array mcrd i in
     let i' = i + 1 in
-    let rb = read_array rowptr i' in
-      sv_float.get j colind mval lb rb
+    let rb = read_array mcrd i' in
+      sv_float.get j mind mval lb rb
 }>.
 
 Tactic Notation "seclocal_fold" := 
@@ -181,77 +182,85 @@ Hypothesis dvec_finite : forall x, In x dvec -> @finite Tdouble x.
 
 Section spmv_monolithic.
 
+(* Product of float-valued sparse CSR matrix and dense vector, implemented
+  without calling any subroutines *)
 Definition spmv := 
   <{
-  fun mval colind rowptr dvec =>
+  fun mval mind mcrd dvec =>
   let "ans" = allocf0 Nrow in
-  let "row_ptr[0]" = read_array rowptr 0 in
+  let "m_crd[0]" = mcrd[0] in
   for i <- [0, Nrow] {
     let s = ref float_unit in
-    let h = read_array rowptr i in
+    let h = mcrd[i] in
     let "i + 1" = i + 1 in
-    let "row_ptr[i + 1]" = read_array rowptr "i + 1" in
-    for j <- [h, "row_ptr[i + 1]"] {
+    let "m_crd[i + 1]" = mcrd["i + 1"] in
+    for j <- [h, "m_crd[i + 1]"] {
       let x = mval[.j] in 
-      let c = colind[j] in 
+      let c = mind[j] in 
       let v = dvec[.c] in 
       fma.func s x v
     };
     let "res" = ! s in
     free s;
-    val_array_set "ans" i "res"
+    "ans"[i] := "res"
   }; 
   "ans"
 }>.
 
 Tactic Notation "seclocal_solver2" :=
-  first [ rewrite /colind_seg list_interval_nth'; auto; solve [ math | seclocal_solver ]
-    | rewrite /colind_seg list_interval_length; auto; solve [ math | seclocal_solver ]
-    | rewrite /colind_seg -list_interval_nth; auto; solve [ math | seclocal_solver ]
-    | idtac ]; auto.
+  solve [ rewrite /mind_seg list_interval_nth'; auto; solve [ math | seclocal_solver ]
+    | rewrite /mind_seg list_interval_length; auto; solve [ math | seclocal_solver ]
+    | rewrite /mind_seg -list_interval_nth; auto; solve [ math | seclocal_solver ]
+    | seclocal_solver; auto
+    | auto using finite_suffcond
+    | auto ].
 
-Lemma spmv_spec `{Inhab (labeled int)} `{Inhab D} (x_mval x_colind x_rowptr x_dvec : loc) : 
-  {{ .arr(x_mval, mval)⟨1, (0,0)⟩ \*
-     arr(x_colind, colind)⟨1, (0,0)⟩ \*
-     arr(x_rowptr, rowptr)⟨1, (0,0)⟩ \*
+Notation "'arrf(' y ',' i 'in' N '=>' f ')⟨' l ',' d '⟩'" := 
+  (harray_fun_float' (fun i => f) y N (LibLabType.Lab (l,0) d)) (at level 32, i binder, format "arrf( y ,  i  in  N  =>  f )⟨ l ,  d ⟩") : hprop_scope.
+    
+(* Specification for `smpv` *)
+Lemma spmv_spec `{Inhab (labeled int)} `{Inhab D} (m_val m_ind m_crd x_dvec : loc) : 
+  {{ .arr(m_val, mval)⟨1, (0,0)⟩ \*
+     arr(m_ind, mind)⟨1, (0,0)⟩ \*
+     arr(m_crd, mcrd)⟨1, (0,0)⟩ \*
      .arr(x_dvec, dvec)⟨1, (0,0)⟩ \* 
-     (\*_(i <- `[0, Nrow] \x `[0, Ncol]) .arr(x_mval, mval)⟨2, i⟩) \*
-     (\*_(i <- `[0, Nrow] \x `[0, Ncol]) arr(x_colind, colind)⟨2, i⟩) \*
-     (\*_(i <- `[0, Nrow] \x `[0, Ncol]) arr(x_rowptr, rowptr)⟨2, i⟩) \*
+     (\*_(i <- `[0, Nrow] \x `[0, Ncol]) .arr(m_val, mval)⟨2, i⟩) \*
+     (\*_(i <- `[0, Nrow] \x `[0, Ncol]) arr(m_ind, mind)⟨2, i⟩) \*
+     (\*_(i <- `[0, Nrow] \x `[0, Ncol]) arr(m_crd, mcrd)⟨2, i⟩) \*
      (\*_(i <- `[0, Nrow] \x `[0, Ncol]) .arr(x_dvec, dvec)⟨2, i⟩) }}
   [{
-    [1| ld in `{(0,0)}                 => spmv x_mval x_colind x_rowptr x_dvec];
-    {2| ld in `[0, Nrow] \x `[0, Ncol] => get x_mval x_colind x_rowptr ld.1 ld.2}
+    [1| ld in `{(0,0)}                 => spmv m_val m_ind m_crd x_dvec];
+    {2| ld in `[0, Nrow] \x `[0, Ncol] => get m_val m_ind m_crd ld.1 ld.2}
   }]
-  {{ hv, 
-  harray_fun_float'  
-    (fun i => (Sum_fma float_unit (lof id Ncol) (fun j => (to_float (hv[`2]((i, j))), dvec[j]))))
-    (hv[`1]((0,0))) Nrow (Lab (1,0) (0,0)) \* \Top }}.
-Proof with (try solve [ seclocal_solver | seclocal_solver2 | auto using finite_suffcond ]; seclocal_fold; try lia).
+  {{ hv,  arrf(
+    hv[`1]((0, 0)), 
+    i in Nrow => Sum_fma float_unit (lof id Ncol) (fun j : int => (to_float (hv[`2]((i, j))), dvec[j])))⟨1, (0, 0)⟩ \* \Top }}.
+                 (* ↑ Coq encoding for a big summation over floating point values *)
+Proof with (try seclocal_solver2; seclocal_fold; try lia).
   xset_Inv Inv 1; xset_R Dom Inv R 2.
-  xin 2 : do 3 (xwp; xapp).
-  xin 1 : (xwp; xapp (@htriple_allocf0_unary)=> // s; xwp; xapp)...
+  xin 2 : xgo.
+  xin 1 : (xwp; xapp (@htriple_allocf0_unary)=> // s; xstep)...
   rewrite prod_cascade.
   xfor_arrayset Inv R R (fun hv i => (Sum_fma float_unit (lof id Ncol) (fun j => (to_float (hv[`2]((i, j))), dvec[j])))) (fun=> float_unit) s.
   { xin 2 : rewrite wp_prod_single /=...
-    xin 1 : (xwp; xapp=> tmp; do 3 (xwp; xapp))...
+    xin 1 : (xstep=> tmp; xgo)...
     xsubst (snd : _ -> int)...
     clear Inv R. xset_Inv Inv 1 tmp. xset_R int Inv R 2%Z.
-    xfocus* 2 (colind_seg l0).
+    xfocus* 2 (mind_seg l0).
     xapp_big sv_float.get_spec_out... 1: case=>??; indomE; autos*.
     xin 1 : idtac.
-    have Hl : length (colind_seg l0) = rowptr[l0 + 1] - rowptr[l0] :> int...
+    have Hl : length (mind_seg l0) = mcrd[l0 + 1] - mcrd[l0] :> int...
     rewrite intr_list ?(fset_of_list_nodup 0) ?Hl ?Union_interval_change2...
     rewrite -> ! hbig_fset_hstar; xclean_heap.
-    xfor_sum Inv R R (fun hv i => (to_float (hv[`2](colind[i])), dvec[colind[i] ])) tmp...
-    { (xin 1: do 3 (xwp; xapp); xapp (@fma.spec)=> y)... 
+    xfor_sum Inv R R (fun hv i => (to_float (hv[`2](mind[i])), dvec[mind[i] ])) tmp...
+    { (xin 1: do 3 xstep; xapp (@fma.spec)=> y)... 
       xapp (@sv_float.get_spec_in)=> //; try math... xsimpl*...
       rewrite list_interval_nth'... }
     { move=> ??? HH. eapply (proj1 (NoDup_nthZ _ _) (nodup_eachcol H1)) in HH... }
-    move=> /= Hfin; xwp; xapp... xwp; xapp; xapp; xsimpl.
+    move=> /= Hfin; xgo... xapp; xsimpl.
     rewrite -/(Sum_fma _ _ _) Sum_fma_lof ?Sum_fma_filter_If'; try intro;
     rewrite -?sorted_bounded_sublist ?Sum_fma_list_interval ?In_lof_id //...
-    move: (indexG0 a0 (colind_seg l0)); rewrite /LibSummation.mem=> ??.
+    move: (indexG0 a0 (mind_seg l0)); rewrite /LibSummation.mem=> ??.
     move=> /[dup] /(nth_index 0){2}<-; rewrite -index_mem=> ?.
     rewrite -list_interval_nth; try apply/(Hfin _ _).1... }
   { apply Sum_fma_feq=>? /In_lof_id ? /= /[! hvE]; indomE... }
